Assume f(x) and g(x) are both [[(1) Differentiable]] at x = a
Then:
| $h(x) = f(x) + g(x)$                 | $h'(a) = f'(a) + g'(a)$           |
| ------------------------------------ | --------------------------------- |
| $h(x) = f(x) g(x)$                   | $h'(a) = f'(a)g(a) + f(a)g'(a)$   |
| $f(a) \ne 0, g(x) = \frac {1}{f(x)}$ | $g'(a) = -\frac{f'(a)}{(f(a))^2}$ |
| $h(x) = \frac {f(x)}{g(x)}$  | $h'(a) = \frac{f'(a)g(a) - f(a)g'(a)}{(g(a)^2)}$                                   |
| $h(x) = f(g(x))$| $h'(a) = f'(g(a))g'(a)$  |                                     |                                   |

