Given a bijection $n: \mathbb{N} \rightarrow \mathbb{N}$ 
	define $b_i := a_{n(i)}$ where now $(b_i)$ is a rearrangement of $(a_n)$


For any $(a_n)$ with@ 
- $a_n \rightarrow 0$
- $\sum_{n: a_n \ge 0} a_n \rightarrow +\infty$
- $\sum_{n: a_n < 0} a_n \rightarrow -\infty$
We can rearrange the [[(1) Series]] $\sum a_n$ to make it [[(3) Converges (Series)]] to any real number


For any $(a_n)$ with:
- $\sum_{n: a_n \ge 0} a_n$ [[(3) Converges (Series)]]
- $\sum_{n: a_n < 0} a_n$ [[(3) Converges (Series)]]
Any rearrangement will give the same sum (since this is just saying that $a_n$ [[(9) Absolutely Converges (Series)]])